start fixing state instantiations
Note:
* Partial progress.

viper-total-heaps/TotalMaskUtil.thy
@@ -5,7 +5,7 @@ theory TotalMaskUtil
 begin
 
 
-subsection \<open>Utilities for \<^typ>\<open>'a nested_mask\<close>\<close>
+subsection \<open>Well-foundness Relation for \<^typ>\<open>'a nested_mask\<close>\<close>
 
 abbreviation nested_mask_rel :: "('a nested_mask \<times> 'a nested_mask) set"
   where "nested_mask_rel \<equiv> {(nm, (NM mh mp fnm)) | nm mh mp fnm ploc. nm \<in> set_option (fnm ploc)}"
@@ -16,11 +16,22 @@ lemma wf_nested_mask_rel: "wf nested_mask_rel"
   apply (rule nested_mask.induct)
   by blast
 
+abbreviation nested_mask_opt_rel :: "('a nested_mask option \<times> 'a nested_mask option) set"
+  where "nested_mask_opt_rel \<equiv>
+    { (Some nm, Some (NM mh mp fnm)) | nm mh mp fnm ploc. nm \<in> set_option (fnm ploc) } \<union>
+    { (None, Some nm) | nm. True } "
+
+lemma wf_nested_mask_opt_rel: "wf nested_mask_opt_rel"
+  sorry
+
+
+subsection \<open>Mask Merge\<close>
+
 fun field_mask_merge :: "field_mask \<Rightarrow> field_mask \<Rightarrow> field_mask" where
-  "field_mask_merge mh\<^sub>1 mh\<^sub>2 = (mh\<^sub>1 +\<lbrakk>(+)\<rbrakk>+ mh\<^sub>2)"
+  "field_mask_merge mh\<^sub>1 mh\<^sub>2 = add_masks mh\<^sub>1 mh\<^sub>2"
 
 fun predicate_mask_merge :: "'a predicate_mask \<Rightarrow> 'a predicate_mask \<Rightarrow> 'a predicate_mask" where
-  "predicate_mask_merge mp\<^sub>1 mp\<^sub>2 = (mp\<^sub>1 +\<lbrakk>(+)\<rbrakk>+ mp\<^sub>2)"
+  "predicate_mask_merge mp\<^sub>1 mp\<^sub>2 = add_masks mp\<^sub>1 mp\<^sub>2"
 
 function (sequential) nested_mask_merge :: "'a nested_mask \<Rightarrow> 'a nested_mask \<Rightarrow> 'a nested_mask" where
   "nested_mask_merge (NM mh\<^sub>1 mp\<^sub>1 fnm\<^sub>1) (NM mh\<^sub>2 mp\<^sub>2 fnm\<^sub>2) =
@@ -43,7 +54,7 @@ text \<open>Defining \<^const>\<open>nested_mask_merge\<close> directly using \<
 declare nested_mask_merge.simps [simp del]
 
 lemma nested_mask_merge_combine_options[simp]:
-  "nested_mask_merge (NM mh\<^sub>1 mp\<^sub>1 nm\<^sub>1) (NM mh\<^sub>2 mp\<^sub>2 nm\<^sub>2) = (NM (mh\<^sub>1 +\<lbrakk>(+)\<rbrakk>+ mh\<^sub>2) (mp\<^sub>1 +\<lbrakk>(+)\<rbrakk>+ mp\<^sub>2) (nm\<^sub>1 +\<lparr>nested_mask_merge\<rparr>+ nm\<^sub>2))"
+  "nested_mask_merge (NM mh\<^sub>1 mp\<^sub>1 nm\<^sub>1) (NM mh\<^sub>2 mp\<^sub>2 nm\<^sub>2) = (NM (add_masks mh\<^sub>1 mh\<^sub>2) (add_masks mp\<^sub>1 mp\<^sub>2) (nm\<^sub>1 +\<lparr>nested_mask_merge\<rparr>+ nm\<^sub>2))"
   unfolding pfun_comb_def combine_options_def
   by (simp add: nested_mask_merge.simps)
 
@@ -70,30 +81,6 @@ fun nested_mask_multiply_option :: "'a nested_mask option \<Rightarrow> preal \<
 | "nested_mask_multiply_option (Some nm) p = (if p = 0 then None else Some (nested_mask_multiply nm p))"
 
 
-subsection \<open>Constant Masks\<close>
-
-fun zero_mh :: "field_mask" where
-  "zero_mh _ = 0"
-
-fun zero_mp :: "'a predicate_mask" where
-  "zero_mp _ = 0"
-
-fun singleton_mh :: "heap_loc \<Rightarrow> preal \<Rightarrow> field_mask" where
-  "singleton_mh loc p l = (if l = loc then p else 0)"
-
-fun singleton_mp :: "'a predicate_loc \<Rightarrow> preal \<Rightarrow> 'a predicate_mask" where
-  "singleton_mp ploc p pl = (if pl = ploc then p else 0)"
-
-fun is_singleton_mh :: "heap_loc \<Rightarrow> field_mask \<Rightarrow> bool" where
-  "is_singleton_mh loc mh = (\<exists>p > 0. mh = singleton_mh loc p)"
-
-fun is_singleton_mp :: "'a predicate_loc \<Rightarrow> 'a predicate_mask \<Rightarrow> bool" where
-  "is_singleton_mp ploc mp = (\<exists>p > 0. mp = singleton_mp ploc p)"
-
-definition empty_nm :: "'a nested_mask"
-  where "empty_nm \<equiv> NM zero_mh zero_mp Map.empty"
-
-
 subsection \<open>Mask Subtraction\<close>
 
 fun field_mask_sub :: "field_mask \<Rightarrow> field_mask \<Rightarrow> field_mask" where
@@ -115,10 +102,52 @@ termination
 subsection \<open>Mask Split\<close>
 
 fun mh_split :: "field_mask \<Rightarrow> field_mask \<Rightarrow> field_mask \<Rightarrow> bool" where
-  "mh_split mh mh\<^sub>1 mh\<^sub>2 = (mh = (mh\<^sub>1 +\<lbrakk>(+)\<rbrakk>+ mh\<^sub>2))"
+  "mh_split mh mh\<^sub>1 mh\<^sub>2 = (mh = add_masks mh\<^sub>1 mh\<^sub>2)"
 
 fun mp_split :: "'a predicate_mask \<Rightarrow> 'a predicate_mask \<Rightarrow> 'a predicate_mask \<Rightarrow> bool" where
-  "mp_split mp mp\<^sub>1 mp\<^sub>2 = (mp = (mp\<^sub>1 +\<lbrakk>(+)\<rbrakk>+ mp\<^sub>2))"
+  "mp_split mp mp\<^sub>1 mp\<^sub>2 = (mp = add_masks mp\<^sub>1 mp\<^sub>2)"
+
+
+subsection \<open>Mask Ordering\<close>
+
+function (sequential) nested_mask_le_opt :: "'a nested_mask option \<Rightarrow> 'a nested_mask option \<Rightarrow> bool" where
+  "nested_mask_le_opt None _ = True"
+| "nested_mask_le_opt _ None = False"
+| "nested_mask_le_opt (Some (NM mh\<^sub>1 mp\<^sub>1 fnm\<^sub>1)) (Some (NM mh\<^sub>2 mp\<^sub>2 fnm\<^sub>2)) =
+     (mh\<^sub>1 \<le> mh\<^sub>2 \<and> mp\<^sub>1 \<le> mp\<^sub>2 \<and> (\<forall>lp. nested_mask_le_opt (fnm\<^sub>1 lp) (fnm\<^sub>2 lp)))"
+  by (pat_completeness) auto
+termination
+  apply (relation "nested_mask_opt_rel <*lex*> {}")
+  using wf_nested_mask_opt_rel
+   apply blast
+  by auto
+
+fun nested_mask_le :: "'a nested_mask \<Rightarrow> 'a nested_mask \<Rightarrow> bool" where
+  "nested_mask_le nm1 nm2 = nested_mask_le_opt (Some nm1) (Some nm2)"
+
+
+subsection \<open>Constant Masks\<close>
+
+fun zero_mh :: "field_mask" where
+  "zero_mh _ = 0"
+
+fun zero_mp :: "'a predicate_mask" where
+  "zero_mp _ = 0"
+
+fun singleton_mh :: "heap_loc \<Rightarrow> preal \<Rightarrow> field_mask" where
+  "singleton_mh loc p l = (if l = loc then p else 0)"
+
+fun singleton_mp :: "'a predicate_loc \<Rightarrow> preal \<Rightarrow> 'a predicate_mask" where
+  "singleton_mp ploc p pl = (if pl = ploc then p else 0)"
+
+fun is_singleton_mh :: "heap_loc \<Rightarrow> field_mask \<Rightarrow> bool" where
+  "is_singleton_mh loc mh = (\<exists>p > 0. mh = singleton_mh loc p)"
+
+fun is_singleton_mp :: "'a predicate_loc \<Rightarrow> 'a predicate_mask \<Rightarrow> bool" where
+  "is_singleton_mp ploc mp = (\<exists>p > 0. mp = singleton_mp ploc p)"
+
+definition empty_nm :: "'a nested_mask"
+  where "empty_nm \<equiv> NM zero_mask zero_mask Map.empty"
 
 
 end
